@prefix geo: <http://www.w3.org/2003/01/geo/wgs84_pos#> .
@prefix owl: <http://www.w3.org/2002/07/owl#> .
@prefix rdf: <http://www.w3.org/1999/02/22-rdf-syntax-ns#> .
@prefix xml: <http://www.w3.org/XML/1998/namespace> .
@prefix xsd: <http://www.w3.org/2001/XMLSchema#> .
@prefix rdfs: <http://www.w3.org/2000/01/rdf-schema#> .
@prefix sigkdd: <http://sigkdd#> .


#################################################################
#
#    Object Properties
#
#################################################################


###  http://sigkdd#award

sigkdd:award rdf:type owl:ObjectProperty ;

       rdfs:comment "The relationship between a person and the award he has been awarded with."@en ;

       rdfs:range sigkdd:Award ;

       rdfs:domain sigkdd:Best_Paper_Awards_Committee ;

       owl:inverseOf sigkdd:awarded_by .



###  http://sigkdd#awarded_by

sigkdd:awarded_by rdf:type owl:ObjectProperty ;

            rdfs:comment "The relationship between an award and the awarded person."@en ;

            rdfs:domain sigkdd:Award ;

            rdfs:range sigkdd:Best_Paper_Awards_Committee .



###  http://sigkdd#can_stay_in

sigkdd:can_stay_in rdf:type owl:ObjectProperty ;

             rdfs:comment "The relationship between a person and a place he can be located at."@en ;

             rdfs:domain sigkdd:Person ;

             rdfs:range sigkdd:Place .



###  http://sigkdd#design

sigkdd:design rdf:type owl:ObjectProperty ;

        rdfs:comment "The relationship between a person or an institution and the entity that has been designed."@en ;

        rdfs:domain sigkdd:ACM_SIGKDD ;

        rdfs:range sigkdd:Deadline ;

        owl:inverseOf sigkdd:designed_by .



###  http://sigkdd#designed_by

sigkdd:designed_by rdf:type owl:ObjectProperty ;

             rdfs:comment "The relationship between the designed entity a the person or an institution that designed it."@en ;

             rdfs:range sigkdd:ACM_SIGKDD ;

             rdfs:domain sigkdd:Deadline .



###  http://sigkdd#hasCommittee

sigkdd:hasCommittee rdf:type owl:ObjectProperty ;

              rdfs:comment "The relation associating a conference with its committees.."@en ;

              rdfs:range sigkdd:Committee ;

              rdfs:domain sigkdd:Conference .



###  http://sigkdd#hasReview

sigkdd:hasReview rdf:type owl:ObjectProperty ;

           rdfs:comment "The relationship linking a paper with its reviewes."@en ;

           rdfs:domain sigkdd:Paper ;

           rdfs:range sigkdd:Review .



###  http://sigkdd#hold

sigkdd:hold rdf:type owl:ObjectProperty ;

      rdfs:comment "The relationship between the person or institution holding an activity."@en ;

      rdfs:domain sigkdd:ACM_SIGKDD ;

      rdfs:range sigkdd:Conference .



###  http://sigkdd#holded_by

sigkdd:holded_by rdf:type owl:ObjectProperty ;

           rdfs:comment "The relationship between the an holded activity and the person or institution holding it."@en ;

           rdfs:range sigkdd:ACM_SIGKDD ;

           rdfs:domain sigkdd:Conference ;

           owl:inverseOf sigkdd:hold .



###  http://sigkdd#isCommitteeOf

sigkdd:isCommitteeOf rdf:type owl:ObjectProperty ;

               rdfs:comment "The relation associating a committee with the conferences."@en ;

               rdfs:domain sigkdd:Committee ;

               rdfs:range sigkdd:Conference .



###  http://sigkdd#isReviewOf

sigkdd:isReviewOf rdf:type owl:ObjectProperty ;

            rdfs:comment "The review associated to a paper."@en ;

            rdfs:domain sigkdd:Review ;

            rdfs:range [ rdf:type owl:Class ;
                         owl:unionOf ( sigkdd:Abstract
                                       sigkdd:Paper
                                     )
                       ] .



###  http://sigkdd#notification_until

sigkdd:notification_until rdf:type owl:ObjectProperty ;

                    rdfs:comment "The relationship between the person or institution to be notified and the deadline for the notification."@en ;

                    rdfs:domain sigkdd:Author ;

                    rdfs:range sigkdd:Deadline_Author_notification .



###  http://sigkdd#obtain

sigkdd:obtain rdf:type owl:ObjectProperty ;

        rdfs:comment "The relationship between a person and the award he has been awarded with."@en ;

        rdfs:domain sigkdd:Author ;

        rdfs:range sigkdd:Award .



###  http://sigkdd#pay

sigkdd:pay rdf:type owl:ObjectProperty ;

     rdfs:comment "The relationship between a person or institution paying an amount of money and the fee for which the money has been payed."@en ;

     rdfs:domain sigkdd:Person ;

     rdfs:range sigkdd:Registration_fee ;

     owl:inverseOf sigkdd:payed_by .



###  http://sigkdd#payed_by

sigkdd:payed_by rdf:type owl:ObjectProperty ;

          rdfs:comment "The relationship between a fee for which the money has been payed and the person or institution paying that amount of money."@en ;

          rdfs:range sigkdd:Person ;

          rdfs:domain sigkdd:Registration_fee .



###  http://sigkdd#presentation

sigkdd:presentation rdf:type owl:ObjectProperty ;

              rdfs:comment "The relationship between the speaker of a presentation and the document that is presented."@en ;

              rdfs:range sigkdd:Document ;

              rdfs:domain sigkdd:Speaker ;

              owl:inverseOf sigkdd:presentationed_by .



###  http://sigkdd#presentationed_by

sigkdd:presentationed_by rdf:type owl:ObjectProperty ;

                   rdfs:comment "The relationship between a document to be presented and the speaker presenting it."@en ;

                   rdfs:domain sigkdd:Document ;

                   rdfs:range sigkdd:Speaker .



###  http://sigkdd#search

sigkdd:search rdf:type owl:ObjectProperty ;

        rdfs:comment "The relationship between the conference organizing association searching for sponsors and a conference sponsor."@en ;

        rdfs:domain sigkdd:ACM_SIGKDD ;

        rdfs:range sigkdd:Sponzor ;

        owl:inverseOf sigkdd:searched_by .



###  http://sigkdd#searched_by

sigkdd:searched_by rdf:type owl:ObjectProperty ;

             rdfs:comment "The relationship between a conference sponsor and the conference organizing association searching for sponsors."@en ;

             rdfs:range sigkdd:ACM_SIGKDD ;

             rdfs:domain sigkdd:Sponzor .



###  http://sigkdd#submit

sigkdd:submit rdf:type owl:ObjectProperty ;

        rdfs:comment "The relationship identyfing the papers submitted by an author,"@en ;

        rdfs:domain sigkdd:Author ;

        rdfs:range sigkdd:Paper .



###  http://sigkdd#submit_until

sigkdd:submit_until rdf:type owl:ObjectProperty ;

              rdfs:comment "The relationship identyfing before which deadline a document is submitted,"@en ;

              rdfs:range sigkdd:Deadline ;

              rdfs:domain sigkdd:Document .





#################################################################
#
#    Data properties
#
#################################################################


###  http://sigkdd#City_of_conference

sigkdd:City_of_conference rdf:type owl:DatatypeProperty ;

                    rdfs:comment "the name of the city in which the conference edition is located." ;

                    rdfs:domain sigkdd:Conference ;

                    rdfs:range xsd:string .



###  http://sigkdd#Currency

sigkdd:Currency rdf:type owl:DatatypeProperty ;

          rdfs:comment "The currency in which the registration fee is expressed."@en ;

          rdfs:domain sigkdd:Fee ;

          rdfs:range xsd:string .



###  http://sigkdd#Date

sigkdd:Date rdf:type owl:DatatypeProperty ;

      rdfs:comment "The date associated with a deadline."@en ;

      rdfs:domain sigkdd:Deadline ;

      rdfs:range xsd:dateTime .



###  http://sigkdd#E-mail

sigkdd:E-mail rdf:type owl:DatatypeProperty ;

        rdfs:comment "The electronic mail address of a person."@en ;

        rdfs:domain sigkdd:Person ;

        rdfs:range xsd:string .



###  http://sigkdd#End_of_conference

sigkdd:End_of_conference rdf:type owl:DatatypeProperty ;

                   rdfs:comment "The ending date of a conference edition."@en ;

                   rdfs:domain sigkdd:Conference ;

                   rdfs:range xsd:dateTime .



###  http://sigkdd#Name

sigkdd:Name rdf:type owl:DatatypeProperty ;

      rdfs:comment "The name of a person."@en ;

      rdfs:domain sigkdd:Person ;

      rdfs:range xsd:string .



###  http://sigkdd#Name_of_conference

sigkdd:Name_of_conference rdf:type owl:DatatypeProperty ;

                    rdfs:comment "The name of a conference."@en ;

                    rdfs:domain sigkdd:Conference ;

                    rdfs:range xsd:string .



###  http://sigkdd#Name_of_sponsor

sigkdd:Name_of_sponsor rdf:type owl:DatatypeProperty ;

                 rdfs:comment "The name of a sponsor."@en ;

                 rdfs:domain sigkdd:Sponzor ;

                 rdfs:range xsd:string .



###  http://sigkdd#Nation

sigkdd:Nation rdf:type owl:DatatypeProperty ;

        rdfs:comment "The nation a person comes from."@en ;

        rdfs:domain sigkdd:Person ;

        rdfs:range xsd:string .



###  http://sigkdd#Price

sigkdd:Price rdf:type owl:DatatypeProperty ;

       rdfs:comment "The registration fee amount."@en ;

       rdfs:domain sigkdd:Fee ;

       rdfs:range xsd:int .



###  http://sigkdd#Start_of_conference

sigkdd:Start_of_conference rdf:type owl:DatatypeProperty ;

                     rdfs:comment "The starting date of a conference edition."@en ;

                     rdfs:domain sigkdd:Conference ;

                     rdfs:range xsd:dateTime .



###  http://sigkdd#hasID

sigkdd:hasID rdf:type owl:DatatypeProperty ;

       rdfs:comment "Numerical identifier, supposed to be unique."@en ;

       rdfs:domain sigkdd:Review ;

       rdfs:range xsd:int .



###  http://sigkdd#hasPostalCode

sigkdd:hasPostalCode rdf:type owl:DatatypeProperty ;

               rdfs:comment "The postal code (ZIP code)."@en ;

               rdfs:domain sigkdd:Place ;

               rdfs:range xsd:int .



###  http://sigkdd#hasStreet

sigkdd:hasStreet rdf:type owl:DatatypeProperty ;

           rdfs:comment "The name of a street."@en ;

           rdfs:domain sigkdd:Place ;

           rdfs:range xsd:string .



###  http://sigkdd#hasText

sigkdd:hasText rdf:type owl:DatatypeProperty ;

         rdfs:domain sigkdd:Review ;

         rdfs:range xsd:string .



###  http://sigkdd#hasTitle

sigkdd:hasTitle rdf:type owl:DatatypeProperty ;

          rdfs:range xsd:string ;

          rdfs:domain [ rdf:type owl:Class ;
                        owl:unionOf ( sigkdd:Abstract
                                      sigkdd:Paper
                                    )
                      ] .



###  http://www.w3.org/2003/01/geo/wgs84_pos#lat

geo:lat rdf:type owl:DatatypeProperty ;

        rdfs:domain sigkdd:Place ;

        rdfs:range xsd:float .



###  http://www.w3.org/2003/01/geo/wgs84_pos#long

geo:long rdf:type owl:DatatypeProperty ;

         rdfs:domain sigkdd:Place ;

         rdfs:range xsd:float .





#################################################################
#
#    Classes
#
#################################################################


###  http://sigkdd#ACM_SIGKDD

sigkdd:ACM_SIGKDD rdf:type owl:Class ;

            rdfs:subClassOf owl:Thing ,
                            [ rdf:type owl:Restriction ;
                              owl:onProperty sigkdd:hold ;
                              owl:someValuesFrom sigkdd:Conference
                            ] ,
                            [ rdf:type owl:Restriction ;
                              owl:onProperty sigkdd:design ;
                              owl:someValuesFrom sigkdd:Deadline
                            ] ,
                            [ rdf:type owl:Restriction ;
                              owl:onProperty sigkdd:search ;
                              owl:someValuesFrom sigkdd:Sponzor
                            ] ;

            rdfs:comment "KDD provides the premier forum for advancement and adoption of the \"science\" of knowledge discovery and data mining"@en .



###  http://sigkdd#Abstract

sigkdd:Abstract rdf:type owl:Class ;

          owl:equivalentClass [ rdf:type owl:Restriction ;
                                owl:onProperty sigkdd:submit_until ;
                                owl:someValuesFrom sigkdd:Deadline_Abstract_Submission
                              ] ;

          rdfs:subClassOf sigkdd:Document ;

          rdfs:comment "The abstract of a paper, that is a brief introduction to its content."@en .



###  http://sigkdd#Author

sigkdd:Author rdf:type owl:Class ;

        owl:equivalentClass [ rdf:type owl:Restriction ;
                              owl:onProperty sigkdd:submit ;
                              owl:someValuesFrom sigkdd:Paper
                            ] ;

        rdfs:subClassOf sigkdd:Speaker ,
                        [ rdf:type owl:Restriction ;
                          owl:onProperty sigkdd:notification_until ;
                          owl:someValuesFrom sigkdd:Deadline_Author_notification
                        ] ;

        rdfs:comment "A person who composes an article, or other written work."@en .



###  http://sigkdd#Author_of_paper

sigkdd:Author_of_paper rdf:type owl:Class ;

                 rdfs:subClassOf sigkdd:Author ,
                                 [ rdf:type owl:Restriction ;
                                   owl:onProperty sigkdd:obtain ;
                                   owl:someValuesFrom sigkdd:Best_Research_Paper_Award
                                 ] ,
                                 [ rdf:type owl:Restriction ;
                                   owl:onProperty sigkdd:obtain ;
                                   owl:someValuesFrom sigkdd:Best_Applications_Paper_Award
                                 ] ;

                 rdfs:comment "A person who composes a paper."@en .



###  http://sigkdd#Author_of_paper_student

sigkdd:Author_of_paper_student rdf:type owl:Class ;

                         rdfs:subClassOf sigkdd:Author ,
                                         [ rdf:type owl:Restriction ;
                                           owl:onProperty sigkdd:obtain ;
                                           owl:someValuesFrom sigkdd:Best_Student_Paper_Award
                                         ] ;

                         rdfs:comment "A student who composes a paper or a senior scientist lightly involved in a paper mainly authored by students."@en .



###  http://sigkdd#Award

sigkdd:Award rdf:type owl:Class ;

       owl:equivalentClass [ rdf:type owl:Restriction ;
                             owl:onProperty sigkdd:awarded_by ;
                             owl:someValuesFrom sigkdd:Organizator
                           ] ;

       rdfs:comment "Something awarded or granted, as for merit"@en .



###  http://sigkdd#Best_Applications_Paper_Award

sigkdd:Best_Applications_Paper_Award rdf:type owl:Class ;

                               rdfs:subClassOf sigkdd:Award ;

                               rdfs:comment "Paper award for the best application"@en .



###  http://sigkdd#Best_Paper_Awards_Committee

sigkdd:Best_Paper_Awards_Committee rdf:type owl:Class ;

                             rdfs:subClassOf sigkdd:Committee ;

                             rdfs:comment "A committee in charge of selecting the best paper to be awarded"@en .



###  http://sigkdd#Best_Research_Paper_Award

sigkdd:Best_Research_Paper_Award rdf:type owl:Class ;

                           rdfs:subClassOf sigkdd:Award ;

                           rdfs:comment "Paper award for the best research paper"@en .



###  http://sigkdd#Best_Student_Paper_Award

sigkdd:Best_Student_Paper_Award rdf:type owl:Class ;

                          rdfs:subClassOf sigkdd:Award ;

                          rdfs:comment "Paper award for the best paper mainly authored by one or more students"@en .



###  http://sigkdd#Best_Student_Paper_Supporter

sigkdd:Best_Student_Paper_Supporter rdf:type owl:Class ;

                              rdfs:subClassOf sigkdd:Sponzor ;

                              rdfs:comment "A sponsor paying for the price of the best student paper."@en .



###  http://sigkdd#Bronze_Supporter

sigkdd:Bronze_Supporter rdf:type owl:Class ;

                  rdfs:subClassOf sigkdd:Sponzor ;

                  rdfs:comment "The entry level for being a sponsor."@en .



###  http://sigkdd#Committee

sigkdd:Committee rdf:type owl:Class ;

           rdfs:comment "A group of people officially delegated to perform a function, such as investigating, considering, reporting, or acting on a matter"@en .



###  http://sigkdd#Conference

sigkdd:Conference rdf:type owl:Class ;

            rdfs:comment "An academic conference or symposium is a conference for researchers (not necessarily academics) to present and discuss their work. Together with academic or scientific journals, conferences provide an important channel for exchange of information between researchers."@en .



###  http://sigkdd#Conference_hall

sigkdd:Conference_hall rdf:type owl:Class ;

                 rdfs:subClassOf sigkdd:Place ;

                 rdfs:comment "A conference hall or conference room is a room provided for singular events such as business conferences and meetings."@en .



###  http://sigkdd#Deadline

sigkdd:Deadline rdf:type owl:Class ;

          rdfs:comment "A time limit for an activity"@en .



###  http://sigkdd#Deadline_Abstract_Submission

sigkdd:Deadline_Abstract_Submission rdf:type owl:Class ;

                              rdfs:subClassOf sigkdd:Deadline ;

                              rdfs:comment "Time limit for abstract submission."@en .



###  http://sigkdd#Deadline_Author_notification

sigkdd:Deadline_Author_notification rdf:type owl:Class ;

                              rdfs:subClassOf sigkdd:Deadline ;

                              rdfs:comment "Time limit for notifying an author about its submitted contribution"@en .



###  http://sigkdd#Deadline_Paper_Submission

sigkdd:Deadline_Paper_Submission rdf:type owl:Class ;

                           rdfs:subClassOf sigkdd:Deadline ;

                           rdfs:comment "Time limit for submitting a paper."@en .



###  http://sigkdd#Document

sigkdd:Document rdf:type owl:Class ;

          rdfs:comment "A writing that contains information."@en .



###  http://sigkdd#Exhibitor

sigkdd:Exhibitor rdf:type owl:Class ;

           rdfs:subClassOf sigkdd:Sponzor ;

           rdfs:comment "A sponsor that organizes an exhibit of its own activities and products."@en .



###  http://sigkdd#Fee

sigkdd:Fee rdf:type owl:Class ;

     rdfs:comment "A fixed sum charged, as by an institution or by law, for a privilege."@en .



###  http://sigkdd#General_Chair

sigkdd:General_Chair rdf:type owl:Class ;

               rdfs:subClassOf sigkdd:Organizator ;

               rdfs:comment "A person with the purpose of overseeing the activities of all conference committee chairs, of ensuring that the objectives of the conference as established by the Steering Committee are met, and of serving as a focal point for communications between the involved entities."@en .



###  http://sigkdd#Gold_Supporter

sigkdd:Gold_Supporter rdf:type owl:Class ;

                rdfs:subClassOf sigkdd:Sponzor ;

                rdfs:comment "An advanced level of sponsorship."@en .



###  http://sigkdd#Hotel

sigkdd:Hotel rdf:type owl:Class ;

       rdfs:subClassOf sigkdd:Place ;

       rdfs:comment "An establishment that provides lodging and usually meals and other services for travelers and other paying guests."@en .



###  http://sigkdd#Invited_Speaker

sigkdd:Invited_Speaker rdf:type owl:Class ;

                 rdfs:subClassOf sigkdd:Speaker ;

                 rdfs:comment "A prominent person required to give a public speech at the conference on a topic of shared interest."@en .



###  http://sigkdd#Listener

sigkdd:Listener rdf:type owl:Class ;

          rdfs:subClassOf sigkdd:Person ;

          rdfs:comment "A person participating at a conference as a listener for others' presentations."@en .



###  http://sigkdd#Main_office

sigkdd:Main_office rdf:type owl:Class ;

             rdfs:subClassOf sigkdd:Place ;

             rdfs:comment "The office that serves as the administrative center of an enterprise or an event."@en .



###  http://sigkdd#Organizator

sigkdd:Organizator rdf:type owl:Class ;

             rdfs:subClassOf sigkdd:Person ;

             rdfs:comment "A person who organizes or is capable of organizing."@en .



###  http://sigkdd#Organizing_Committee

sigkdd:Organizing_Committee rdf:type owl:Class ;

                      rdfs:subClassOf sigkdd:Committee ;

                      rdfs:comment "The Local Organizing Committee is charged with the planning and direction of all (non-scientific) program facets of the conference including selection of venue. The Organizing Committee is responsible for planning and executing all financial aspects of the Conference and reports to the Executive Committee. The Local Organizing Committee shall include representatives of the host country and/or institution."@en .



###  http://sigkdd#Organizing_Committee_member

sigkdd:Organizing_Committee_member rdf:type owl:Class ;

                             rdfs:subClassOf sigkdd:Organizator ;

                             rdfs:comment "A person that is part of the organizing committee."@en .



###  http://sigkdd#Paper

sigkdd:Paper rdf:type owl:Class ;

       owl:equivalentClass [ rdf:type owl:Restriction ;
                             owl:onProperty sigkdd:submit_until ;
                             owl:someValuesFrom sigkdd:Deadline_Paper_Submission
                           ] ;

       rdfs:subClassOf sigkdd:Document ;

       rdfs:comment "A scientific article around a subject of interest."@en .



###  http://sigkdd#Person

sigkdd:Person rdf:type owl:Class ;

        owl:equivalentClass [ rdf:type owl:Restriction ;
                              owl:onProperty sigkdd:pay ;
                              owl:someValuesFrom sigkdd:Registration_fee
                            ] ;

        rdfs:subClassOf owl:Thing ,
                        [ rdf:type owl:Restriction ;
                          owl:onProperty sigkdd:can_stay_in ;
                          owl:someValuesFrom sigkdd:Hotel
                        ] ;

        rdfs:comment "An individual human being."@en .



###  http://sigkdd#Place

sigkdd:Place rdf:type owl:Class ;

       rdfs:comment "A building or an area set aside for a specified purpose."@en .



###  http://sigkdd#Platinum_Supporter

sigkdd:Platinum_Supporter rdf:type owl:Class ;

                    rdfs:subClassOf sigkdd:Sponzor ;

                    rdfs:comment "The most advanced level of sponsorship."@en .



###  http://sigkdd#Program_Chair

sigkdd:Program_Chair rdf:type owl:Class ;

               rdfs:subClassOf sigkdd:Organizator ;

               rdfs:comment "A person that is in charge of overseeing the activities of all Program Committee members in putting together a technical program which supports the objectives of the conference, and producing the conference proceedings."@en .



###  http://sigkdd#Program_Committee

sigkdd:Program_Committee rdf:type owl:Class ;

                   rdfs:subClassOf sigkdd:Committee ;

                   rdfs:comment "The Scientific Committee has the following responsibilities: suggesting keynote speakers and approving the Organising Committee’s final list of keynote speakers; Approving the Organising Committee’s proposal concerning section profiles and titles; Reviewing abstracts after initial review by the Organising Committee; Giving feedback to the Organising Committee on the proposed programme; Adhering to the deadlines agreed to with the Organising Committee; Participating in the event"@en .



###  http://sigkdd#Program_Committee_member

sigkdd:Program_Committee_member rdf:type owl:Class ;

                          rdfs:subClassOf sigkdd:Organizator ;

                          rdfs:comment "A member of the program committee."@en .



###  http://sigkdd#Registration_Non-Member

sigkdd:Registration_Non-Member rdf:type owl:Class ;

                         rdfs:subClassOf sigkdd:Registration_fee ;

                         rdfs:comment "Registration fee for person not member of SIGKDD organization."@en .



###  http://sigkdd#Registration_SIGKDD_Member

sigkdd:Registration_SIGKDD_Member rdf:type owl:Class ;

                            rdfs:subClassOf sigkdd:Registration_fee ;

                            rdfs:comment "Registration fee for person that are member of SIGKDD organization."@en .



###  http://sigkdd#Registration_SIGMOD_Member

sigkdd:Registration_SIGMOD_Member rdf:type owl:Class ;

                            rdfs:subClassOf sigkdd:Registration_fee ;

                            rdfs:comment "Registration fee for person that are member of SIGMOD organization."@en .



###  http://sigkdd#Registration_Student

sigkdd:Registration_Student rdf:type owl:Class ;

                      rdfs:subClassOf sigkdd:Registration_fee ;

                      rdfs:comment "Registration fee for students, usually at a reduced price."@en .



###  http://sigkdd#Registration_fee

sigkdd:Registration_fee rdf:type owl:Class ;

                  rdfs:subClassOf sigkdd:Fee ;

                  rdfs:comment "Fee requested for registering and participating at a conference."@en .



###  http://sigkdd#Review

sigkdd:Review rdf:type owl:Class ;

        rdfs:subClassOf sigkdd:Document ;

        rdfs:comment "The document with the outcome of a read through of a paper in order to correct possible errors and formulate a judgement on the quality of the work and appropriateness for the intended conference."@en .



###  http://sigkdd#Silver_Supporter

sigkdd:Silver_Supporter rdf:type owl:Class ;

                  rdfs:subClassOf sigkdd:Sponzor ;

                  rdfs:comment "A mid-level for sponsorhip."@en .



###  http://sigkdd#Speaker

sigkdd:Speaker rdf:type owl:Class ;

         owl:equivalentClass [ rdf:type owl:Restriction ;
                               owl:onProperty sigkdd:presentation ;
                               owl:someValuesFrom sigkdd:Document
                             ] ;

         rdfs:subClassOf sigkdd:Person ;

         rdfs:comment "A person participating at a conference as a speaker in an activity involving an oral presentation,"@en .



###  http://sigkdd#Sponzor

sigkdd:Sponzor rdf:type owl:Class ;

         owl:equivalentClass [ rdf:type owl:Restriction ;
                               owl:onProperty sigkdd:pay ;
                               owl:someValuesFrom sigkdd:Sponzor_fee
                             ] ;

         rdfs:comment "A commercial organization that pays all or part of the cost of putting on an event."@en .



###  http://sigkdd#Sponzor_fee

sigkdd:Sponzor_fee rdf:type owl:Class ;

             rdfs:subClassOf sigkdd:Fee ;

             rdfs:comment "The fee that sponsor need to pay to be considered as such."@en .



###  http://sigkdd#Webmaster

sigkdd:Webmaster rdf:type owl:Class ;

           rdfs:subClassOf sigkdd:Organizator ;

           rdfs:comment "A person whose occupation is designing, developing, marketing, or maintaining websites."@en .





#################################################################
#
#    Annotations
#
#################################################################


sigkdd:Reviewer rdfs:comment "One who reviews, especially one who writes reviews for correcting errors and ensuring quality."@en .




###  Generated by the OWL API (version 3.5.0) http://owlapi.sourceforge.net
